<?xml version='1.0' encoding='utf-8'?>

<section xml:id="PS4" xmlns:xi="http://www.w3.org/2001/XInclude" tbil-slides="build">
  <title>Taylor Series (PS4)</title>
    <objectives>
        <ul>
            <li>
                <xi:include href="outcomes/04.ptx"/>
            </li>
        </ul>
    </objectives>
  <subsection>
    <title>Activities</title>
    
    
    
    <activity>
        <introduction>
            <p>
                The following tasks will help us find a mechanism to produce
                a power series given information about its derivatives.
            </p>
        </introduction>
        <task>
            <p>
                Find the 2nd derivative of <m>x^2</m>.
            </p>
            <ol marker='A' cols="2">
                <li><m>2x</m></li>
                <li><m>2</m></li>
                <li><m>4x</m></li>
                <li><m>4</m></li>
            </ol>
        </task>
        
        <task>
            <p>
                Find the 3rd derivative of <m>x^3</m>.
            </p>
            <ol marker='A' cols="2">
                <li><m>2</m></li>
                <li><m>3x</m></li>
                <li><m>6</m></li>
                <li><m>12x</m></li>
            </ol>
        </task>
        
        <task>
            <p>
                Find the 4th derivative of <m>x^4</m>.
            </p>
            <ol marker='A' cols="2">
                <li><m>18</m></li>
                <li><m>24</m></li>
                <li><m>32</m></li>
                <li><m>64</m></li>
            </ol>
        </task>
        
        <task>
            <p>
                Based on these results, which of the following should always
                equal the <m>n</m>th derivative of <m>x^n</m> with respect to <m>x</m>?
            </p>
            <ol marker='A' cols="2">
                <li><m>n</m></li>
                <li><m>n^2</m></li>
                <li><m>n!</m></li>
                <li><m>n^n</m></li>
            </ol>
        </task>
        
        <!-- <task>
            <p>
                What then is the <m>(n+1)</m>th derivative of <m>f(x)=x^n</m> with respect to <m>x</m>?
            </p>
            <ol marker='A' cols="2">
                <li><m>0</m></li>
                <li><m>1</m></li>
                <li><m>2n</m></li>
                <li><m>(n-1)!</m></li>
            </ol>
        </task> -->
        
    </activity>
    
    <activity>
        <introduction>
            <p>
                Let's use derivatives to rediscover the sequence <m>a_n</m> which gives
                a power series representation for <m>e^x</m>.
            </p>
        </introduction>
        <task>
            <p>
            Let's say that
                <me>e^x=\sum_{n=0}^\infty a_nx^n=a_0+a_1x+a_2x^2+a_3x^3+a_4x^4\dots</me>.
            </p>
            <p>
                What must <m>a_0</m> be to satisfy <m>e^0=1</m>?
            </p>
        </task>
        
        <task>
            <p>
                Then, <me>\frac{d}{dx}[e^x]=e^x=a_1+2a_2x+3a_3x^2+4a_4x^3\dots</me>.
            </p>
            <p>
                What must <m>a_1</m> be to also satisfy <m>e^0=1</m>?
            </p>
        </task>
        
        
        <task>
            <p>
                Then, <me>\frac{d^2}{dx^2}[e^x]=e^x=2a_2+6a_3x+12a_4x^2+\dots</me>.
            </p>
            <p>
                What must <m>a_2</m> be to also satisfy <m>e^0=1</m>?
            </p>
        </task>
        
        
        <task>
            <p>
                Then, <me>\frac{d^3}{dx^3}[e^x]=e^x=6a_3+24a_4x+\dots</me>.
            </p>
            <p>
                What must <m>a_3</m> be to also satisfy <m>e^0=1</m>?
            </p>
        </task>
        
        
        <task>
            <p>
                So this <m>6a_3</m> term was obtained from the fact that the <m>3</m>rd
                derivative of <m>x^3</m> is <m>3!=6</m>.
            </p>
            <p>
                So finally, we may skip ahead to the <m>n</m>th derivative:
                <me>\frac{d^n}{dx^n}[e^x]=e^x=n!\cdot a_n+(n+1)!\cdot a_{n+1}\cdot x+\dots</me>.
            </p>
            <p>
                What must <m>a_n</m> be to also satisfy <m>e^0=1</m>?
            </p>
        </task>
        
        
        <task>
            <p>
                This reveals the power series we previously found for <m>e^x</m>:
                <me>e^x=\sum_{n=0}^\infty a_nx^n=\sum_{n=0}^\infty \frac{1}{n!}x^n</me>.
            </p>
            <p>
                So in general, if <m>f(x)=a_0+a_1x+a_2x^2+\dots</m>,
                then <me>\frac{d^n}{dx^n}[f(x)]=f^{(n)}(x)=n!\cdot a_n+(n+1)!\cdot a_{n+1}\cdot x+\dots</me>.
            </p>
            <p>
                What must <m>a_n</m> be to produce the correct value for <m>f^{(n)}(0)</m>?
            </p>
        </task>
        
    </activity>
    
    
    
<!--     
    <activity xml:id="activity-PS4taylorSeriesExist">
        <introduction>
            <p>
Suppose <m>f</m> is a function.
Then if <m>f(x)</m> can be represented as a power series, there is a real number <m>c</m> and an interval, <m>I</m>,
centered at <m>x=c</m> such that <m>f(x)=\displaystyle\sum_{n=0}^\infty a_n(x-c)^n=a_0+a_1(x-c)+a_2(x-c)^2+a_3(x-c)^3+\ldots</m> on <m>I</m>.
            </p>
        </introduction>
        <task>
            <p>
                Use term-by-term differentiation to find a power series for <m>f^\prime(x)</m>.
            </p>
        </task>
        <task>
            <p>
                Use this power series to find <m>f'(c)</m>.
            </p>
        </task>
        <task>
            <p>
                Use term-by-term differentiation to find a power series for <m>f^{\prime\prime}(x)</m>.
            </p>
        </task>
        
         <task>
            <p>
                Use this power series to find <m>f''(c)</m>.
            </p>
        </task>
        
        
        <task>
            <p>
                Use term-by-term differentiation to find a power series for <m>f^{\prime\prime\prime}(x)</m>.
            </p>
        </task>
        
         <task>
            <p>
                Use this power series to find <m>f'''(c)</m>.
            </p>
        </task>
        
        <task>
            <p>
                Deduce that <m>f^{(n)}(c)=n!a_n</m> and hence <m>a_n=\displaystyle\frac{f^{(n)}(c)}{n!}</m>.
            </p>
        </task>
    </activity> -->
    
    
    
    <fact xml:id="fact-PS4taylorSeriesForm">
          <statement>
      <p>
        If <m>f(x)</m> can be written as a power series, then there is a real number <m>c</m> such that
          <md>
          <mrow>f(x)&amp;=\sum_{n=0}^\infty \frac{f^{(n)}(c)}{n!}(x-c)^n</mrow>
          <mrow>&amp;=f(c)+f^\prime(c)(x-c)+\frac{f^{\prime\prime}(c)}{2!}(x-c)^2+\frac{f^{(3)}(c)}{3!}(x-c)^3+\ldots</mrow>
          </md>
          on some interval centered at <m>x=c</m>.
      </p>
      <p>
        In fact, the functions that can be represented as power series are exactly those functions which 
        are infinitely differentiable on some open interval.
      </p>
              </statement>
        </fact>
    
    <definition xml:id="definition-PS4taylorSeries">
            <statement>
                <p>
                    The <term>Taylor series</term><idx>Taylor Series</idx> generated by <m>f(x)</m> and
                    <em>centered</em> at <m>x=c</m> is given by
          <md>
          <mrow>f(x)&amp;=\sum_{n=0}^\infty \frac{f^{(n)}(c)}{n!}(x-c)^n</mrow>
          <mrow>&amp;=f(c)+f^\prime(c)(x-c)+\frac{f^{\prime\prime}(c)}{2!}(x-c)^2+\frac{f^{(3)}(c)}{3!}(x-c)^3+\ldots</mrow>
          </md>
                    with an interval of convergence determinable by series convergence rules.
                </p>
                <p>
When <m>c=0</m>, 
          <md>
          <mrow>f(x)&amp;=\sum_{n=0}^\infty \frac{f^{(n)}(0)}{n!}x^n</mrow>
          <mrow>&amp;=f(0)+f^\prime(0)x+\frac{f^{\prime\prime}(0)}{2!}x^2+\frac{f^{(3)}(0)}{3!}x^3+\ldots</mrow>
          </md>
is called the <term>Maclaurin series</term><idx>Maclaurin Series</idx> generated by <m>f</m>.
                </p>
            </statement>
        
        </definition>

<activity>
    <introduction>
        <p>
            Observe that <m>f(x)=\sin(x)</m> is a function such that:
            
            <me>
                \begin{array}{c|c|c|c|c|c|c|c}
                f(0) &amp; f'(0) &amp; f''(0) &amp; f^{(3)}(0) &amp; f^{(4)}(0) &amp; f^{(5)}(0) &amp; f^{(6)}(0) &amp; f^{(7)}(0) \\
                \hline
                \sin(0) &amp; \cos(0) &amp; -\sin(0) &amp; -\cos(0) &amp; \sin(0) &amp; \cos(0) &amp; -\sin(0) &amp; -\cos(0) \\
                \hline
                0 &amp; 1 &amp; 0 &amp; -1 &amp; 0 &amp; 1 &amp; 0 &amp; -1
                \end{array}
            </me></p></introduction>
            
    <task>
        <p>Given the zeros appearing for every even derivative above, 
        which of these is a valid simplification of the Maclarin series
        <m>\displaystyle\sum_{n=0}^\infty\frac{f^{(n)}(0)}{n!}x^n</m> for <m>\sin(x)</m>?</p>
            <ol marker='A' cols="2">
                <li><m>\sum_{n=1}^\infty\frac{f^{(n)}(0)}{n!}x^n</m></li>
                <li><m>\sum_{2n=0}^\infty\frac{f^{(n)}(0)}{n!}x^n</m></li>
                <li><m>\sum_{n=0}^\infty\frac{f^{(2n)}(0)}{(2n)!}x^{2n}</m></li>
                <li><m>\sum_{n=0}^\infty\frac{f^{(2n+1)}(0)}{(2n+1)!}x^{2n+1}</m></li>
            </ol>
    </task>     
    <task>
        <p>Now consider
        the following consolidated chart:
          <me>
                \begin{array}{c|c|c|c|c|c|c|c}
                f^{(1)}(0) &amp; f^{(3)}(0) &amp;f^{(5)}(0) &amp; f^{(7)}(0) \\
                \hline
                \cos(0) &amp; -\cos(0) &amp;  \cos(0) &amp; -\cos(0) \\
                \hline
                 1 &amp;  -1 &amp; 1 &amp;  -1
                \end{array}
            </me></p>
        <p>Which formula yields these alternating <m>1</m>s and <m>-1</m>s
        appearing for <m>f^{(2n+1)}(0)</m>?
        </p>
            <ol marker='A' cols="2">
                <li><m>f^{(2n+1)}(0)=(-1)^n</m></li>
                <li><m>f^{(2n+1)}(0)=(-1)^{n+1}</m></li>
                <li><m>f^{(2n+1)}(0)=(-1)^{2n}</m></li>
                <li><m>f^{(2n+1)}(0)=(-1)^{2n+1}</m></li>
            </ol>
    </task> 
</activity>

<fact xml:id="fact-maclaurin-series-common">
    <statement>
        <p>
            The power series we've introduced for each of the following functions
            are in fact their Maclaurin series (Taylor series centered at <m>0</m>).
        </p>
        <md>
            <mrow>\frac{1}{1-x} = \sum_{n=0}^\infty \frac{n!}{n!}x^n\amp= 1+x+x^2+x^3+\dots</mrow>
            <mrow>e^x = \sum_{n=0}^\infty \frac{1}{n!}x^n\amp= 1+x+\frac{x^2}{2}+\frac{x^3}{6}+\dots</mrow>
            <mrow>\cos(x)= \sum_{n=0}^\infty \frac{(-1)^n}{(2n)!}x^{2n}\amp =1-\frac{x^2}{2}+\frac{x^4}{24}-\frac{x^6}{720}+\dots</mrow>
            <mrow>\sin(x)=\displaystyle \sum_{n=0}^\infty \frac{(-1)^n}{(2n+1)!}x^{2n+1}\amp =x-\frac{x^3}{6}+\frac{x^5}{120}-\frac{x^7}{5040}+\dots</mrow>
        </md>
    </statement>
</fact>
    
    
    <definition xml:id="definition-PS4taylorPolynomial">
            <statement>
                <p>
                For a function <m>f(x)</m> with a Taylor series centered at <m>x=c</m>,
                    <md>
                    <mrow>f(x) \amp\approx T_k(x)</mrow>
                    <mrow>\amp = \sum_{n=0}^k \frac{f^{(n)}(c)}{n!}(x-c)^n </mrow>
                    <mrow>\amp = f(c)+f^\prime(c)(x-c)+\frac{f^{\prime\prime}(c)}{2!}(x-c)^2+
                    <!-- \frac{f^{(3)}(c)}{3!}(x-c)^3+ -->
                    \ldots+\frac{f^{(k)}(c)}{k!}(x-c)^k</mrow>
                        </md>
        where <m>T_k(x)</m> is called the <m>k^{th}</m> degree
        <term>Taylor polynomial</term><idx>Taylor polynomial</idx> generated by <m>f</m> and centered at <m>x=c</m>.
                </p>
                <p>
The <m>k^{th}</m> degree Taylor polynomial can be seen as the <q>best</q> polynomial of degree <m>k</m> or less for approximating <m>f(x)</m> for values close to <m>x=c</m>.
Note that  the <m>1^{st}</m> degree Taylor polynomial is also known as the <term>linearization</term><idx>linearization of a function</idx> of <m>f</m>.
                </p>
            </statement>
        </definition>
    
<activity checkit-seed="2301" checkit-slug="PS4" checkit-title="Taylor series">
    <introduction>
        <p>
            Let <m>f(x)</m> be a function such that:
            
            <me>
                \begin{array}{c|c|c|c|c|c|c}
                f(4) &amp; f'(4) &amp; f''(4) &amp; f'''(4) &amp; f^{(4)}(4) &amp; f^{(5)}(4) &amp; f^{(6)}(4) \\
                \hline
                0 &amp; 1 &amp; 2 &amp; 3 &amp; 4 &amp; 5 &amp; 6 
                \end{array}
            </me></p></introduction>
            
            
    <task><p>Find a Taylor polynomial for <m>f(x)</m> centered at <m>x=4</m> of degree <m>3</m>.</p></task>
    <task><p>Using the table above, find a general closed form for <m>f^{(n)}(4)</m>.</p></task>
    <task><p>Use (b) to find a Taylor series for <m>f(x)</m> centered at <m>x=4</m>.</p></task>
            
 <!--   <answer>
            <ol>
                <li><m>f_{ 3 }(x)=\frac{1}{2} \, {\left(x - 4\right)}^{3} + {\left(x - 4\right)}^{2} + x - 4</m>.</li>
                <li><m>f^{(n)}(4)=n</m>.</li>
                <li><m>\displaystyle f(x)=\sum_{n=0}^\infty \frac{ n }{n!} (x-4)^n</m>.</li>
            </ol>
    </answer>-->
</activity>    

<activity checkit-seed="2486" checkit-slug="PS4" checkit-title="Taylor series">
    <introduction>
        <p>
            Let <m>f(x)</m> be a function such that:
            
            <me>
                \begin{array}{c|c|c|c|c|c|c}
                f(-2) &amp; f'(-2) &amp; f''(-2) &amp; f'''(-2) &amp; f^{(4)}(-2) &amp; f^{(5)}(-2) &amp; f^{(6)}(-2) \\
                \hline
                0 &amp; 2 &amp; -16 &amp; 54 &amp; -128 &amp; 250 &amp; -432 
                \end{array}
            </me></p></introduction>
            
           
    <task><p>Find a Taylor polynomial for <m>f(x)</m> centered at <m>x=-2</m> of degree <m>3</m>.</p></task>
    <task><p>Using the table above, find a general closed form for <m>f^{(n)}(-2)</m>.</p></task>
    <task><p>Use (b) to find a Taylor series for <m>f(x)</m> centered at <m>x=-2</m>.</p></task>
  
  <!--  <answer>
            <ol>
                <li><m>f_{ 3 }(x)=9 \, {\left(x + 2\right)}^{3} - 8 \, {\left(x + 2\right)}^{2} + 2 \, x + 4</m>.</li>
                <li><m>f^{(n)}(-2)=-2 \, \left(-1\right)^{n} n^{3}</m>.</li>
                <li><m>\displaystyle f(x)=\sum_{n=0}^\infty \frac{ -2 \, \left(-1\right)^{n} n^{3} }{n!} (x-(-2))^n</m>.</li>
            </ol>
    </answer>-->
</activity>    
    
    <!-- <activity xml:id="activity-PS4sineCosineExponential">
        
        <task>
            <p>
                Find the Maclaurin series for <m>f(x)=\sin(x)</m> about <m>x=0</m>, along with the interval of validity.
            </p>
        </task>
        <task>
            <p>
                Find the Taylor series generated by <m>f(x)=\cos(x)</m> about <m>x=0</m>.
            </p>
        </task>
        
        <task>
            <p>
                Find the Maclaurin series for <m>f(x)=e^x</m> about <m>x=0</m>, along with the interval of validity.
            </p>
        </task>
    </activity> -->
    
    
    <remark>
        <statement>
        <p>
            You might have seen <m>\sqrt{-1}</m> written as <m>i</m>, and know that <m>z</m> is a complex number if <m>z=a+bi</m> for some real numbers <m>a</m> and <m>b</m>.
Note that <m>i^2=-1</m>, <m>i^3=(i^2)i=-i</m>, <m>i^4=(i^2)^2=1</m>, <m>i^5=(i^4)i=i</m>, and so on.
This gives rise to the following notion.
        </p>
    </statement>
    </remark>
        
    
       <definition xml:id="definition-PS4eulerIdentity">
           <title>Euler's Identity</title>
            <statement>
                <p>
                    For any real number <m>\theta</m>,
                
                
                <md>
                    <mrow>e^{i\theta}  &amp; =  1+\displaystyle\frac{i\theta}{1!}+\displaystyle\frac{(i\theta)^2}{2!}+\displaystyle\frac{(i\theta)^3}{3!}+\displaystyle\frac{(i\theta)^4}{4!}+\displaystyle\frac{(i\theta)^5}{5!}+\displaystyle\frac{(i\theta)^6}{6!}+\displaystyle\frac{(i\theta)^7}{7!}+\displaystyle\frac{(i\theta)^8}{8!}+\ldots</mrow>
                    <mrow>&amp; =  1+i\theta-\displaystyle\frac{\theta^2}{2!}-\displaystyle\frac{i\theta^3}{3!}+\displaystyle\frac{\theta^4}{4!}+\displaystyle\frac{i\theta^5}{5!}-\displaystyle\frac{\theta^6}{6!}-\displaystyle\frac{i\theta^7}{7!}+\displaystyle\frac{\theta^8}{8!}+\ldots</mrow>
                    <mrow>&amp; =  \left(1-\displaystyle\frac{\theta^2}{2!}+\displaystyle\frac{\theta^4}{4!}-\displaystyle\frac{\theta^6}{6!}+\ldots\right)+i\left(\theta-\displaystyle\frac{\theta^3}{3!}+\displaystyle\frac{\theta^5}{5!}-\displaystyle\frac{\theta^7}{7!}+\ldots\right)</mrow>
                    <mrow>&amp; =  \cos(\theta)+i\sin(\theta).</mrow>
                </md>

<!--<m>e^{i\theta}  =  1+\displaystyle\frac{i\theta}{1!}+\displaystyle\frac{(i\theta)^2}{2!}+\displaystyle\frac{(i\theta)^3}{3!}+\displaystyle\frac{(i\theta)^4}{4!}+\displaystyle\frac{(i\theta)^5}{5!}+\displaystyle\frac{(i\theta)^6}{6!}+\displaystyle\frac{(i\theta)^7}{7!}+\displaystyle\frac{(i\theta)^8}{8!}+\ldots
 =  1+i\theta-\displaystyle\frac{\theta^2}{2!}-\displaystyle\frac{i\theta^3}{3!}+\displaystyle\frac{\theta^4}{4!}+\displaystyle\frac{i\theta^5}{5!}-\displaystyle\frac{\theta^6}{6!}-\displaystyle\frac{i\theta^7}{7!}+\displaystyle\frac{\theta^8}{8!}+\ldots
 =  \left(1-\displaystyle\frac{\theta^2}{2!}+\displaystyle\frac{\theta^4}{4!}-\displaystyle\frac{\theta^6}{6!}+\ldots\right)+i\left(\theta-\displaystyle\frac{\theta^3}{3!}+\displaystyle\frac{\theta^5}{5!}-\displaystyle\frac{\theta^7}{7!}+\ldots\right)
 =  \cos(\theta)+i\sin(\theta)</m>.-->
                </p>
                
            </statement>
        
        </definition>
    
    
    
        <activity xml:id="activity-PS4eulerIdentityExample">
            <statement>
               <p>
                   Use Euler's identity to evaluate <m>e^{i\pi}</m>.
               </p>
           </statement>
       </activity>
    
    
       <activity xml:id="activity-PS4eulerIdentityExample2">
           <statement>
              <p>
                  Use Euler's identity to evaluate <m>e^{i\pi/2}</m>.
              </p>
          </statement>
      </activity>
    
    
      <activity xml:id="activity-PS4eulerIdentityExample3">
          <statement>
             <p>
                Use the result of <xref ref="activity-PS4eulerIdentityExample2"/> to evaluate <m>i^i=(\unknown)^i</m>.
             </p>
         </statement>
     </activity>
    
    
    
    <!-- <subsection>
        <title>Slideshow</title>
        <p>Slideshow of activities available at <url href="PS4.slides.html"/>.</p>
    </subsection> -->
    
    </subsection>
    <subsection>
        <title>Videos</title>
    <figure>
		<video xml:id="video-PS4" youtube="bjktfFCafGs">
			<!--<track kind="subtitles" label="US English" xml:lang="en" source="videos/E1-captions.vtt" default=""/>-->
		</video>
        <caption>Video: Determine a Taylor or Maclaurin series for a function



</caption>
    </figure>
         
        
        
    </subsection>
    
    
    
    
    
    
    
    
    
    
    
</section>

 