<?xml version='1.0' encoding='utf-8'?>

<section xml:id="SQ3" xmlns:xi="http://www.w3.org/2001/XInclude" tbil-slides="build">
  <title>Partial Sum Sequence (SQ3)</title>
    <objectives>
        <ul>
            <li>
                <xi:include href="outcomes/03.ptx"/>
            </li>
        </ul>
    </objectives>
  <subsection>
    <title>Activities</title>
    <activity xml:id="activity-SQ3intropartialsumsgeometric">
        <introduction>
            <p>
                Consider the sequence <m>\displaystyle \{a_n\}_{n=0}^\infty=\left\{\frac{1}{2^n}\right\}_{n=0}^\infty</m>.
            </p>
        </introduction>
        <task>
            <p>
                Find the first 5 terms of this sequence.
            </p>
        </task>
        <task>
            <p>
                Compute the following:
                <ol>
                    <li><m>a_0.</m></li>
                    <li><m>a_0+a_1.</m></li>
                    <li><m>a_0+a_1+a_2.</m></li>
                    <li><m>a_0+a_1+a_2+a_3.</m></li>
                    <li><m>a_0+a_1+a_2+a_3+a_4.</m></li>
                </ol>
            </p>
        </task>
    </activity>
    
    <activity xml:id="activity-SQ3intropartialsumsharmonic">
        <introduction>
            <p>
                Consider the sequence <m>\displaystyle \{a_n\}_{n=1}^\infty=\left\{\frac{1}{n}\right\}_{n=1}^\infty</m>.
            </p>
        </introduction>
        <task>
            <p>
                Find the first 5 terms of this sequence.
            </p>
        </task>
        <task>
            <p>
                Compute the following:
                <ol>
                    <li><m>a_1.</m></li>
                    <li><m>a_1+a_2.</m></li>
                    <li><m>a_1+a_2+a_3.</m></li>
                    <li><m>a_1+a_2+a_3+a_4.</m></li>
                    <li><m>a_1+a_2+a_3+a_4+a_5.</m></li>
                </ol>
            </p>
        </task>
    </activity>
        
        <definition xml:id="definition-SQ3partialsumsequence">
            <statement>
                <p>
                    Given a sequence <m>\{a_n\}_{n=0}^\infty</m> define the <em><m>k^{\text{th}}</m> partial sum</em> of <m>\{a_n\}</m> to be <me>A_k=\sum_{i=0}^k a_i=a_1+a_2+\cdots+a_k.</me>  Note that <m>\{A_n\}=A_0, A_1, A_2, \ldots</m> is itself a sequence called the <em>partial sum sequence</em>.
                </p>
            </statement>
        </definition>
        
        <activity xml:id="activity-SQ3geompartialsum">
            <statement>
                <p>
                     Let <m>a_n=\frac{2}{3^n}.</m> Find the following partial sums:
                    <ol>
                        <li><m>A_0</m>.</li>
                        <li><m>A_1</m>.</li>
                        <li><m>A_2</m>.</li>
                        <li><m>A_3</m>.</li>
                        <li><m>A_{100}</m>.</li>
                    </ol>
                </p>
                 
            </statement>
        </activity>
        
        <activity xml:id="activity-SQ3closedformmotivation">
            <statement>
                <p>Consider the sequence <m>a_n=\frac{2}{3^n}.</m> What is the best way to find the 100th partial sum <m>A_{100}</m>?
                    <ol marker="A." cols="2">
                        <li>Sum the first 101 terms of the sequence <m>\{a_n\}</m>.</li>
                        <li>Find a closed form for the partial sum sequence <m>\{A_n\}</m>.</li>
                    </ol>
                </p>
            </statement>
        </activity>
        
        <activity xml:id="activity-SQ3polyproducts">
            <statement>
                <p>Expand the following polynomial products, and then reduce to as few summands as possible.
                    <ol>
                        <li><m>(1-x)(1+x+x^2)</m>.</li>
                        <li><m>(1-x)(1+x+x^2+x^3)</m>.</li>
                        <li><m>(1-x)(1+x+x^2+x^3+x^4)</m>.</li>
                        <li><m>(1-x)(1+x+x^2+\cdots+x^n)</m>, where <m>n</m> is any nonnegative integer.</li>
                    </ol>
                </p>
            </statement>
        </activity>
        
        <activity xml:id="activity-SQ3simplifyingsum">
            <statement>
                <p>Suppose <m>\displaystyle S_5=1+\frac{1}{2}+\frac{1}{4}+\frac{1}{8}+\frac{1}{16}+\frac{1}{32}.</m>  Without actually computing this sum, which of the following is equal to <m>\left(1-\frac{1}{2}\right)S_5</m>?
                    <ol marker="A." cols="1">
                        <li><m>\displaystyle\frac{1}{2}+\frac{1}{4}+\frac{1}{8}+\frac{1}{16}+\frac{1}{32}-\frac{1}{64}</m>.</li>
                        <li><m>\displaystyle1-\frac{1}{64}</m>.</li>
                        <li><m>\displaystyle1-\frac{1}{2}-\frac{1}{4}-\frac{1}{8}-\frac{1}{16}-\frac{1}{32}</m>.</li>
                    </ol>
                </p>
            </statement>
        </activity>
        
        <activity xml:id="activity-SQ3particularclosedform">
            <introduction>
                <p>
                    Recall from <xref ref="activity-SQ3geompartialsum"/> that <m>\displaystyle A_{100}=2+\frac{2}{3}+\frac{2}{3^2}+\frac{2}{3^3}+\frac{2}{3^4}+\cdots+\frac{2}{3^{100}}=2\left(1+\frac{1}{3}+\frac{1}{3^2}+\frac{1}{3^3}+\frac{1}{3^4}+\cdots+\frac{1}{3^{100}}\right).</m> 
                </p>
            </introduction>
            <task>
                <p>
                     Which of the following is equal to <m>\displaystyle\left(1-\frac{1}{3}\right)A_{100}</m>?
                    <ol marker="A." cols="2">
                        <li><m>\displaystyle1-\frac{1}{3^{101}}</m>.</li>
                        <li><m>\displaystyle1-\frac{1}{3^{100}}</m>.</li>
                        <li><m>\displaystyle2\left(1-\frac{1}{3^{101}}\right)</m>.</li>
                        <li><m>\displaystyle2\left(1-\frac{1}{3^{100}}\right)</m>.</li>
                    </ol>
                </p>
            </task>
            <task>
                <p>
                    Based on your previous choice, write out an expression for <m>A_{100}</m>.
                </p>
            </task>
                    
        </activity>
        
        <activity xml:id="activity-SQ3nthclosedform">
            <introduction>
                <p>
                    Suppose that <m>\displaystyle \{b_n\}_{n=0}^\infty=\{(-2)^n\}_{n=0}^\infty=\{1,-2,4,-8,\ldots\}</m>.  Let <m>B_n=\displaystyle\sum_{i=0}^n b_i</m> be the <m>n</m>th partial sum of <m>\{b_n\}</m>.  
                </p>
            </introduction>
            <task>
                <p>
                     Find simple expressions for the following:
                    <ol>
                        <li><m>(1-(-2))B_{10}</m>.</li>
                        <li><m>(1-(-2))B_{30}</m>.</li>
                        <li>
                            <p><m>(1-(-2))B_{n}</m>. Choose from the following:</p>
                            <ol marker="A." cols="2">
                                <li><m>1+(-2)^n</m>.</li>
                                <li><m>1-(-2)^n</m>.</li>
                                <li><m>1+(-2)^{n+1}</m>.</li>
                                <li><m>1-(-2)^{n+1}</m>.</li>
                                <li><m>1-2^n</m>.</li>
                            </ol>
                        </li>
                    </ol>
                </p>
            </task>
            <task>
                <p>
                    Based on your previous answers, solve for the following:
                    <ol>
                        <li><m>B_{10}</m>.</li>
                        <li><m>B_{30}</m>.</li>
                        <li>
                            <p><m>B_{n}</m>. Choose from the following:</p>                            
                            <ol marker="A." cols="2">
                                <li><m>\displaystyle \frac{1-(-2)^{n+1}}{1-(-2)}</m></li>
                                <li><m>\displaystyle \frac{1-(-2)^{n+1}}{1-2}</m></li>
                                <li><m>\displaystyle \frac{1-(-2)^{n+1}}{1+(-2)}</m></li>
                                <li><m>\displaystyle \frac{1-(-2)^{n}}{1-2}</m></li>
                                <li><m>\displaystyle \frac{1-(-2)^{n}}{1-(-2)}</m></li>
                            </ol>
                        </li>
                    </ol>
                </p>
            </task>
                    
        </activity>
        
        <activity xml:id="activity-SQ3closedformgeomhandsoff">
            <introduction>
                <p>
                    Consider the following sequences:
                    <ol>
                        <li><m>\displaystyle\{a_n\}_{n=0}^\infty=\left\{\left(-\frac{2}{3}\right)^n\right\}_{n=0}^\infty</m>.</li>
                        <li><m>\displaystyle\{b_n\}_{n=0}^\infty=\left\{2\cdot\left(-1\right)^n\right\}_{n=0}^\infty</m>.</li>
                        <li><m>\displaystyle\{c_n\}_{n=0}^\infty=\left\{-3\cdot \left(1.2\right)^n\right\}_{n=0}^\infty</m>.</li>
                    </ol>
                </p>
            </introduction>
            <task>
                <p>
                    Find the closed form for the <m>n</m>th partial sum for the geometric sequence <m>A_n=\displaystyle\sum_{i=0}^n a_i=\displaystyle\sum_{i=0}^n \left(-\frac{2}{3}\right)^n</m>.
                    <ol marker="A." cols="2">
                        <li><m>\displaystyle \frac{3}{5}\left(1-\left(-\frac{2}{3}\right)^{n+1}\right)</m>.</li>
                        <li><m>\displaystyle \frac{5}{3}\left(1-\left(-\frac{2}{3}\right)^{n+1}\right)</m>.</li>
                        <li><m>\displaystyle \frac{5}{3}\left(1+\frac{2}{3}\left(\frac{2}{3}\right)^{n}\right)</m>.</li>
                        <li><m>\displaystyle \frac{3}{5}\left(1+\frac{2}{3}\left(\frac{2}{3}\right)^{n}\right)</m>.</li>
                        <li><m>\displaystyle 1-\left(-\frac{2}{3}\right)^{n+1}</m>.</li>
                    </ol>
                </p>
            </task>
            <task>
                <p>
                    Find the closed form for the <m>n</m>th partial sum for the geometric sequence <m>B_n=\displaystyle\sum_{i=0}^n b_i=\displaystyle\sum_{i=0}^n 2\cdot\left(-1\right)^n</m>.
                    <ol marker="A." cols="2">
                        <li><m>\displaystyle 2^{n+1}</m>.</li>
                        <li><m>\displaystyle 1-(-1)^{n+1}</m>.</li>
                        <li><m>\displaystyle 1+(-1)^{n}</m>.</li>
                        <li><m>\displaystyle 2(1+(-1)^{n})</m>.</li>
                        <li><m>\displaystyle 2(1-(-1)^{n+1})</m>.</li>
                    </ol>
                </p>
            </task>
            <task>
                <p>
                    Find the closed form for the <m>n</m>th partial sum for the geometric sequence <m>C_n=\displaystyle\sum_{i=0}^n c_i=\displaystyle\sum_{i=0}^n -3\cdot \left(1.2\right)^n</m>.
                </p>            
            </task>
          </activity>
            <activity>
                <p>
                    Given the closed forms you found in <xref ref="activity-SQ3closedformgeomhandsoff"/>, which of the following limits are defined?  If defined, what is the limit?
                    <ol marker="A." cols="2">
                        <li><m>\displaystyle\lim_{n\to\infty}A_n</m>.</li>
                        <li><m>\displaystyle\lim_{n\to\infty}B_n</m>.</li>
                        <li><m>\displaystyle\lim_{n\to\infty}C_n</m>.</li>
                    </ol>
                </p>
            </activity>
        
        <definition xml:id="definition-SQ3serieslimit">
            <statement>
                <p>
                    Given a sequence <m>a_n</m>, we define the limit of the series <me>\displaystyle\sum_{n=k}^\infty a_n:=\lim_{n\to \infty} A_n</me> where <m>A_n=\displaystyle \sum_{i=k}^n a_i</m>.  We call <m>\displaystyle\sum_{n=k}^\infty a_n</m> an <em>infinite series</em>.
                </p>
            </statement>
        </definition>
        
        <activity xml:id="activity-SQ3geomserieslimit">
            <statement>
                <p>
                    Which of the following series are infinite?
                    <ol marker="A." cols="2">
                        <li><m>\displaystyle\sum_{n=0}^\infty 3(0.8)^n</m>.</li>
                        <li><m>\displaystyle\sum_{n=0}^\infty 2\left(\frac{5}{4}\right)^n</m>.</li>
                        <li><m>\displaystyle\sum_{n=0}^\infty \left(\frac{5}{6}\right)^n</m>.</li>
                        <li><m>\displaystyle\sum_{n=0}^\infty \frac{1}{2}\left(81\right)^n</m>.</li>
                        <li><m>\displaystyle\sum_{n=0}^\infty 10\left(-\frac{1}{5}\right)^n</m>.</li>
                    </ol>
                </p>
            </statement>
        </activity>
        
        
        <activity xml:id="activity-SQ3telescopingpartialsums">
            <statement>
                <p>
                    Let <m>\displaystyle\{a_n\}_{n=1}^\infty=\left\{\frac{1}{n}-\frac{1}{n+1}\right\}=1-\frac{1}{2}, \frac{1}{2}-\frac{1}{3}, \frac{1}{3}-\frac{1}{4},\ldots</m>.  Let <m>\displaystyle A_n=\sum_{i=1}^na_i=\sum_{i=1}^n \left(\frac{1}{i}-\frac{1}{i+1} \right)</m>.
                </p>
                <p>
                    Which of the following is the best strategy for evaluating <m>\displaystyle A_{4}=\left(1-\frac{1}{2} \right)+\left(\frac{1}{2}-\frac{1}{3} \right)+\left(\frac{1}{3}-\frac{1}{4} \right)+\left(\frac{1}{4}-\frac{1}{5} \right)</m>?
                    <ol marker="A.">
                        <li>Compute <m>\displaystyle A_{4}=\left(1-\frac{1}{2} \right)+\left(\frac{1}{2}-\frac{1}{3} \right)+\left(\frac{1}{3}-\frac{1}{4} \right)+\left(\frac{1}{4}-\frac{1}{5} \right)=\frac{1}{2}+\frac{1}{6}+\frac{1}{12}+\frac{1}{20}</m>, then evaluate the sum.</li>
                        <li>Rewrite <m>\displaystyle A_{4}=\left(1-\frac{1}{2} \right)+\left(\frac{1}{2}-\frac{1}{3} \right)+\left(\frac{1}{3}-\frac{1}{4} \right)+\left(\frac{1}{4}-\frac{1}{5} \right)=1+\left(-\frac{1}{2}+\frac{1}{2}\right)+\left(-\frac{1}{3}+\frac{1}{3}\right)+\left(-\frac{1}{4}+\frac{1}{4}\right)-\frac{1}{5}</m>, then simplify.</li>
                    </ol>
                </p>
            </statement>
        </activity>
        
        
        <activity xml:id="activity-SQ3telescopingpartialsumsclosed">
            <statement>
                <p>
                    Recall from <xref ref="activity-SQ3telescopingpartialsums"/> that <m>\displaystyle\{a_n\}_{n=1}^\infty=\left\{\frac{1}{n}-\frac{1}{n+1}\right\}</m> and <m>\displaystyle A_n=\sum_{i=1}^na_i=\sum_{i=1}^n \left(\frac{1}{i}-\frac{1}{i+1} \right)</m>.
                </p>
                <p>
                    Compute the following partial sums:
                    <ol>
                        <li><m>A_3</m>.</li>
                        <li><m>A_{10}</m>.</li>
                        <li><m>A_{100}</m>.</li>
                    </ol>
                </p>
            </statement>
        </activity>
        
        
        <activity xml:id="activity-SQ3telescopingclosedform">
            <statement>
                <p>
                    Recall from <xref ref="activity-SQ3telescopingpartialsums"/> that <m>\displaystyle\{a_n\}_{n=1}^\infty=\left\{\frac{1}{n}-\frac{1}{n+1}\right\}</m> and <m>\displaystyle A_n=\sum_{i=1}^na_i=\sum_{i=1}^n \left(\frac{1}{i}-\frac{1}{i+1} \right)</m>.
                </p>
                <p>
                    Which of the following is equal to <m>A_n</m>?
                    <ol marker="A." cols="2">
                        <li><m>n-\frac{1}{n+1}</m>.</li>
                        <li><m>1-\frac{1}{n}</m>.</li>
                        <li><m>1-\frac{1}{n+1}</m>.</li>
                        <li><m>1-\frac{1}{i}</m>.</li>
                        <li><m>1-\frac{1}{i+1}</m>.</li>
                    </ol>
                </p>
            </statement>
        </activity>
        
        
        <definition xml:id="definition-SQ3telescoping">
            <statement>
                <p>
                    Given a sequence <m>\{x_n\}_1^\infty</m> and a sequence of the form <m>\{s_n\}_1^\infty:=\{x_n-x_{n+1}\}_1^\infty</m>  we call the series <m>S_n=\displaystyle\sum_{i=1}^n s_i=\sum_{i=1}^n(x_i-x_{i+1})</m> to be a <em>telescoping series</em>.
                </p>
            </statement>
        </definition>
        
        <activity xml:id="activity-SQ3generaltelescoping">
            <statement>
                <p>
                    Given a telescoping series <m>S_n=\displaystyle\sum_{i=1}^n s_i=\sum_{i=1}^n(x_i-x_{i+1})</m>, find:
                    <ol>
                        <li><m>S_2</m>.</li>
                        <li><m>S_{10}</m>.</li>
                        <li>
                            <p>Choose <m>S_{n}</m> from the following options:</p>                            
                            <ol marker="A." cols="2">
                                <li><m>x_1-x_n</m></li>
                                <li><m>x_1-x_{n+1}</m></li>
                                <li><m>x_1-x_{n-1}</m></li>
                                <li><m>x_1-x_n+1</m></li>
                                <li><m>x_1-x_n-1</m></li>
                            </ol>
                         </li>
                    </ol>
                </p>
            </statement>
        </activity>
        
        
        
        <activity xml:id="activity-SQ3telescopinghandsoff">
                <p>
                    For each of the following telescoping series, find the closed form for the <m>n</m>th partial sum.
                    <ol>
                        <li><m>S_n=\displaystyle\sum_{i=1}^n (2^{-i}-(2^{-i-1}))</m>.</li>
                        <li><m>S_n=\displaystyle\sum_{i=1}^n (i^2-(i+1)^2)</m>.</li>
                        <li><m>S_n=\displaystyle\sum_{i=1}^n \left( \frac{1}{2i+1}-\frac{1}{2i+3}\right)</m>.</li>
                    </ol>
                </p>
        </activity>
    
        <activity>
            <p>Given the closed forms you found in <xref ref="activity-SQ3telescopinghandsoff"/>, determine which of the following telescoping series converge. If so, to what value does it converge?</p>
                    <ol marker="A." cols="2">
                        <li><m>\displaystyle\sum_{i=1}^\infty (2^{-i}-(2^{-i-1}))</m>.</li>
                        <li><m>\displaystyle\sum_{i=1}^\infty (i^2-(i+1)^2)</m>.</li>
                        <li><m>\displaystyle\sum_{i=1}^\infty \left( \frac{1}{2i+1}-\frac{1}{2i+3}\right)</m>.</li>
                    </ol>            
        </activity>

<activity checkit-seed="3192" checkit-slug="SQ3" checkit-title="Partial sum sequence">
    <introduction>
       
        <p>Consider the partial sum sequence <m>\displaystyle A_n=\left(-2\right)+\left(\frac{2}{3}\right)+\left(-\frac{2}{9}\right)+\cdots+\left(-2\cdot \left( -\frac{1}{3}\right)^n \right).</m></p></introduction>
                    
                        <task><p>Find a closed form for <m>A_n</m>.</p></task>
                        <task><p>Does <m>\{A_n\}</m> converge?  If so, to what value?</p></task>
    </activity>
    <activity>
 
         <introduction>
             <p>Consider the partial sum sequence <m>\displaystyle B_n=\sum_{i=1}^n \left( \frac{1}{5 \, i + 2}-\frac{1}{5 \, i + 7} \right).</m></p></introduction>
                    
                        <task><p>Find a closed form for <m>B_n</m>.</p></task>
                        <task><p>Does <m>\{B_n\}</m> converge?  If so, to what value?</p></task>
                    
 <!--   <answer>
        <p>
            <ol>
                <li>
                    <ol>
                        <li><m>\displaystyle A_n=-2\cdot\frac{1-\left(-\frac{1}{3}\right)^{n+1} }{1- \left(-\frac{1}{3}\right) }</m>.</li>
                        <li>
                            <m>\displaystyle\lim_{n\to\infty} -2\cdot\frac{1-\left(-\frac{1}{3}\right)^{n+1} }{1- \left(-\frac{1}{3}\right) } </m> converges to <m>-\frac{3}{2}</m>.                
                        </li>            
                    </ol>
                </li>
                <li>
                    <ol>
                        <li><m>\displaystyle B_n=\frac{1}{7}-\frac{1}{5 \, n + 7}</m>.</li>
                        <li>
                            <m>\displaystyle\lim_{n\to\infty} \frac{1}{7}-\frac{1}{5 \, n + 7} </m> converges to <m>\frac{1}{7}</m>.                
                        </li>            
                    </ol>
                </li>
            </ol>
        </p>
    </answer>-->
</activity>
    
    <!-- <subsection>
        <title>Slideshow</title>
        <p>Slideshow of activities available at <url href="SQ3.slides.html"/>.</p>
    </subsection> -->
    </subsection>
    <subsection>
        <title>Videos</title>
    <figure>
		<video xml:id="video-SQ3" youtube="RHqnvkBtGZA">
			<!--<track kind="subtitles" label="US English" xml:lang="en" source="videos/E1-captions.vtt" default=""/>-->
		</video>
        <caption>Video: Compute the first few terms of a telescoping or geometric partial sum sequence, and find a closed form for this sequence, and compute its limit.

</caption>
    </figure>
         
        
        
    </subsection>
        
    
</section>
